ebpf/Asm.v
@@ -19,6 +19,7 @@ Require Import Locations.
 
 Require Import Conventions Events Smallstep.
 Require Stacklayout.
+Require Import Op.
 
 (** * Abstract syntax *)
 
@@ -69,6 +70,8 @@ Definition preg_of (r: mreg) : preg :=
   | D0 => FR F0 | D1 => FR F1 | D2 => FR F2
   end.
 
+Declare Scope asm.
+
 (** Conventional names for stack pointer ([SP]) *)
 
 Notation "'SP'" := R10 (only parsing) : asm.
@@ -88,12 +91,17 @@ Definition label := positive.
 
 Inductive width := W32 | W64.
 
-Inductive immw : width -> Type :=
+(*Inductive immw : width -> Type :=
 | Imm32  : forall (i:int), immw W32
 | Imm64  : forall (i:int64), immw W64.
-
+*)
 
 Definition warchi := if Archi.ptr64 then W64 else W32.
+
+Inductive conv :=
+| DWOFW (* long of int *)
+| WOFDW (* int of long *)
+.
 
 Inductive aluOp : Type :=
   | ADD   (**r dst += src *)
@@ -108,7 +116,9 @@ Inductive aluOp : Type :=
   | MOD   (**r dst %= src *)
   | XOR   (**r dst ^= src *)
   | MOV   (**r dst = src *)
-  | ARSH. (**r dst >>= src (signed) *)
+  | ARSH  (**r dst >>= src (signed) *)
+  | CONV (c:conv)  (**r dst = src *)
+.
 
 Inductive cmpOp : Type :=
   | EQ: cmpOp                (**r e1 == e2 *)
@@ -138,12 +148,13 @@ Definition sizew (s:sizeOp) :=
   end.
 
 Inductive instruction : Type :=
+  | Pmov  : forall (dst:ireg) (cst:int64), instruction   (** dst = cst *)
   | Pload : forall (sz:sizeOp) (dst:ireg) (src:ireg) (offset:off), instruction        (** dst = * (size) (src + offset) *)
-  | Pstore : forall (sz:sizeOp) (dst:ireg) (src:ireg+immw (sizew sz)) (offset:off), instruction   (**r * (size) (dst + offset) = src *)
-  | Palu : forall (o:aluOp) (w:width) (r:ireg) (a:ireg+immw w), instruction    (**r arithmetics *)
-  | Pcmp : forall (o:cmpOp) (w:width) (r:ireg) (a:ireg+immw w), instruction             (**r comparison without branching: eBPF extension *)
+  | Pstore : forall (sz:sizeOp) (dst:ireg) (src:ireg+int) (offset:off), instruction   (**r * (size) (dst + offset) = src *)
+  | Palu : forall (o:aluOp) (w:width) (r:ireg) (a:ireg+int), instruction    (**r arithmetics *)
+  | Pcmp : forall (o:cmpOp) (w:width) (r:ireg) (a:ireg+int), instruction             (**r comparison without branching: eBPF extension *)
   | Pjmp : ident+label -> instruction                           (**r unconditional jump *)
-  | Pjmpcmp : forall (o:cmpOp) (w:width) (r:ireg) (a:ireg+immw w) (l:label), instruction (**r conditional jump with comparison *)
+  | Pjmpcmp : forall (o:cmpOp) (w:width) (r:ireg) (a:ireg+int) (l:label), instruction (**r conditional jump with comparison *)
   | Pcall : ireg+ident -> signature -> instruction              (**r function call *)
   | Pret : instruction                                          (**r function return *)
 
@@ -174,7 +185,6 @@ Definition genv := Genv.t fundef unit.
 
 Notation "a # b" := (a b) (at level 1, only parsing) : asm.
 Notation "a # b <- c" := (Pregmap.set b c a) (at level 1, b at next level) : asm.
-
 Open Scope asm.
 
 (** Undefining some registers *)
@@ -265,51 +275,79 @@ Definition goto_label (f: function) (lbl: label) (rs: regset) (m: mem) :=
       end
   end.
 
+Definition int64_of_intu (i:int) := Int64.repr (Int.unsigned i).
 
-Definition eval_reg_immw (w:width) (rs : regset) (ri: ireg+immw w) : val :=
+Definition int64_is_intu (n:int64) :=
+  let i := Int64.unsigned n in
+  Z.leb i Int.max_unsigned.
+
+
+Definition map_sum_left {A B A': Type} (F: A -> A')  (x: A+B) : A'+B :=
+  match x with
+  | inl i => inl (F i)
+  | inr i => inr i
+  end.
+
+Definition eval_reg_immw (w:width) (rs : regset) (ri: ireg+int) : val :=
   match ri with
-  | inl i => (fun i0 : ireg => rs i0) i
-  | inr i =>
-      match i with
-      | Imm32 i => Vint i
-      | Imm64 i => Vlong i
-      end
+  | inl i => rs i
+  | inr i => match w with
+             | W32 => Vint i
+             | W64 => Vlong (int64_of_intu i)
+             end
+  end.
+
+
+Definition eval_val_int (w:width)  (ri: val+int) : val :=
+  match ri with
+  | inl i =>  i
+  | inr i => match w with
+             | W32 => Vint i
+             | W64 => Vlong (int64_of_intu i) (* constant are given an unsigned interpretation *)
+             end
   end.
 
 (** Evaluation of [Palu] operands *)
-
-Definition eval_alu (b: aluOp) (w:width) (v1 v2: val) : option val :=
+Definition eval_alu (b: aluOp) (w:width) (v1:val) (v2: val+int) : option val :=
   match b with
-  | ADD => Some (if w then Val.add v1 v2 else Val.addl v1 v2)
-  | SUB => Some (if w then Val.sub v1 v2 else Val.subl v1 v2)
-  | MUL => Some (if w then Val.mul v1 v2 else Val.mull v1 v2)
-  | DIV => if w then Val.divu v1 v2 else Val.divlu v1 v2
-  | OR  => Some (if w then Val.or v1 v2 else Val.orl v1 v2)
-  | AND => Some (if w then Val.and v1 v2 else Val.andl v1 v2)
-  | LSH => Some (if w then Val.shl v1 v2 else Val.shll v1 v2)
-  | RSH => Some (if w then Val.shru v1 v2 else Val.shrlu v1 v2)
-  | NEG => Some (if w then Val.neg v2 else Val.negl v2)
-  | MOD => if w then Val.modu v1 v2 else Val.modlu v1 v2
-  | XOR => Some (if w then Val.xor v1 v2 else Val.xorl v1 v2)
-  | MOV => Some v2
-  | ARSH => Some (if w then Val.shr v1 v2 else Val.shrl v1 v2)
+  | ADD => Some ((if w then Val.add else Val.addl) v1 (eval_val_int w v2))
+  | SUB => Some ((if w then Val.sub else Val.subl) v1 (eval_val_int w v2))
+  | MUL => Some ((if w then Val.mul else Val.mull) v1 (eval_val_int w v2))
+  | DIV => (if w then Val.divu else Val.divlu) v1 (eval_val_int w v2)
+  | OR  => Some ((if w then Val.or else Val.orl) v1 (eval_val_int w v2))
+  | AND => Some ((if w then Val.and else Val.andl) v1 (eval_val_int w v2))
+  | LSH => Some ((if w then Val.shl else Val.shll) v1 (eval_val_int W32 v2))
+  | RSH => Some ((if w then Val.shru else Val.shrlu) v1 (eval_val_int W32 v2))
+  | NEG => Some ((if w then Val.neg else Val.negl) (eval_val_int w v2))
+  | MOD => (if w then Val.modu else Val.modlu) v1 (eval_val_int w v2)
+  | XOR => Some ((if w then Val.xor else Val.xorl) v1 (eval_val_int w v2))
+  | MOV => Some (eval_val_int w v2)
+  | ARSH => Some ((if w then Val.shr else Val.shrl) v1 (eval_val_int W32 v2))
+  | CONV DWOFW  => Some (Val.longofintu v1) (* v1 & FF_FF_FF_FF *)
+  | CONV WOFDW  => Some (Val.loword v1)     (* v1 & FF_FF_FF_FF *)
   end.
 
 (** Evaluation of [Pcmp] and [Pjmpcmp] operands *)
 
-Definition eval_cmp (op: cmpOp) (w:width) (rs: regset) (m: mem) (r: ireg) (ri: ireg+immw w) : option bool :=
+Definition cmpu (w:width) :=
+  if w then Val.cmpu_bool else Val.cmplu_bool.
+
+Definition cmp (w:width) :=
+  if  w then Val.cmp_bool else Val.cmpl_bool.
+
+Definition eval_cmp (op: cmpOp) (w:width) (rs: regset) (m: mem) (r: ireg) (ri: ireg+int) : option bool :=
   match op with
-  | EQ          => Val.cmpu_bool (Mem.valid_pointer m) Ceq (rs#r) (eval_reg_immw w rs ri)
-  | GT Signed   => Val.cmp_bool Cgt (rs#r) (eval_reg_immw w rs ri)
-  | GT Unsigned => Val.cmpu_bool (Mem.valid_pointer m) Cgt (rs#r) (eval_reg_immw w rs ri)
-  | GE Signed   => Val.cmp_bool Cge (rs#r) (eval_reg_immw w rs ri)
-  | GE Unsigned => Val.cmpu_bool (Mem.valid_pointer m) Cge (rs#r) (eval_reg_immw w rs ri)
-  | LT Signed   => Val.cmp_bool Clt (rs#r) (eval_reg_immw w rs ri)
-  | LT Unsigned => Val.cmpu_bool (Mem.valid_pointer m) Clt (rs#r) (eval_reg_immw w rs ri)
-  | LE Signed   => Val.cmp_bool Cle (rs#r) (eval_reg_immw w rs ri)
-  | LE Unsigned => Val.cmpu_bool (Mem.valid_pointer m) Cle (rs#r) (eval_reg_immw w rs ri)
-  | SET         => Val.cmpu_bool (Mem.valid_pointer m) Cne (Val.and (rs#r) (eval_reg_immw w rs ri)) (Vint Int.zero)
-  | NE          => Val.cmpu_bool (Mem.valid_pointer m) Cne (rs#r) (eval_reg_immw w rs ri)
+  | EQ          => (cmpu w) (Mem.valid_pointer m) Ceq (rs#r) (eval_reg_immw w rs ri)
+  | GT Signed   => (cmp w) Cgt (rs#r) (eval_reg_immw w rs ri)
+  | GT Unsigned => (cmpu w) (Mem.valid_pointer m) Cgt (rs#r) (eval_reg_immw w rs ri)
+  | GE Signed   => (cmp w) Cge (rs#r) (eval_reg_immw w rs ri)
+  | GE Unsigned => (cmpu w) (Mem.valid_pointer m) Cge (rs#r) (eval_reg_immw w rs ri)
+  | LT Signed   => (cmp w) Clt (rs#r) (eval_reg_immw w rs ri)
+  | LT Unsigned => (cmpu w) (Mem.valid_pointer m) Clt (rs#r) (eval_reg_immw w rs ri)
+  | LE Signed   => (cmp w) Cle (rs#r) (eval_reg_immw w rs ri)
+  | LE Unsigned => (cmpu w) (Mem.valid_pointer m) Cle (rs#r) (eval_reg_immw w rs ri)
+  | SET         => (cmpu w) (Mem.valid_pointer m) Cne (Val.and (rs#r) (eval_reg_immw w rs ri)) (Vint Int.zero)
+  | NE          => (cmpu w) (Mem.valid_pointer m) Cne (rs#r) (eval_reg_immw w rs ri)
   end.
 
 
@@ -367,14 +405,14 @@ Definition store (k: sizeOp) (addr:val) (v:val) (m:mem) :=
   end.
 
 
-Definition exec_store (k: sizeOp) (r:ireg) (ri:ireg+immw (sizew k)) (o:Ptrofs.int) (rs: regset) (m:mem) :=
+Definition exec_store (k: sizeOp) (r:ireg) (ri:ireg+int) (o:Ptrofs.int) (rs: regset) (m:mem) :=
   match store  k (Val.offset_ptr rs#r o) (eval_reg_immw (sizew k) rs ri) m with
   | None => Stuck
   | Some m' => Next (nextinstr rs) m'
   end.
 
-Definition exec_alu (o: aluOp) (w:width) (r: ireg) (ri: ireg+immw w) (rs: regset) (m: mem) :=
-  match eval_alu o w (rs#r) (eval_reg_immw w rs ri) with
+Definition exec_alu (o: aluOp) (w:width) (r: ireg) (ri: ireg+int) (rs: regset) (m: mem) :=
+  match eval_alu o w (rs#r) (map_sum_left (fun (x:ireg) => rs#x) ri) with
   | None => Stuck
   | Some v => Next (nextinstr (rs#r <- v)) m
   end.
@@ -398,6 +436,7 @@ Definition exec_branch (f: function) (l: label) (rs: regset) (m: mem) (res: opti
 
 Definition exec_instr (f: function) (i: instruction) (rs:regset) (m: mem) : outcome :=
   match i with
+  | Pmov r v        => Next (nextinstr (rs#r <- (Vlong v))) m
   | Pload k r r' o   => exec_load k r r' o rs m
   | Pstore k r ri o  => exec_store k r ri o rs m
   | Palu o w r ri      => exec_alu o w r ri rs m
